Add transport as syymbol

src/reflection.v
@@ -218,42 +218,19 @@ Lemma uniqueness :
     Ttt.isterm Γ u T1 ->
     Ttt.isterm Γ u T2 ->
     Ttt.eqtype Γ T1 T2.
+Admitted.
 
-Definition transport n T1 T2 p t : term :=
-  let s    := Uni (uni n) in
-  let w    := sbweak s in
-  let wT1  := Subst T1 w in
-  let ws   := Subst s w in
-  let ww   := sbweak (Id ws wT1 (var 0)) in
-  let wwT1 := Subst wT1 ww in
-
-  app (j s T1 (Arrow wwT1 (var 1)) (lam T1 (Subst T1 (sbweak T1)) (var 0)) T2 p)
-      T1 (* -> *) T2
-      t.
-
-Lemma TermTransport :
-  forall {Γ n T1 T2 p t},
-    Ttt.isctx Γ ->
-    Ttt.isterm Γ T1 (Uni (uni n)) ->
-    Ttt.isterm Γ T2 (Uni (uni n)) ->
-    Ttt.isterm Γ p (Id (Uni (uni n)) T1 T2) ->
-    Ttt.isterm Γ t T1 ->
-    Ttt.isterm Γ (transport n T1 T2 p t) T2.
-Proof.
-  intros Γ n T1 T2 p t ? ? ? ? ?.
-  unfold transport, Ttt.isterm.
-  assert (Ttt.istype Γ T1).
-  { replace T1 with (El (uni n) T1) by reflexivity.
-    unfold Ttt.istype. magic.
-  }
-  (* magic. *)
-  ceapply TermTyConv ; [ ceapply TermApp | .. ].
-  - ceapply TermTyConv ; [ ceapply TermJ | .. ].
-    + magic.
-    + magic.
-    + ceapply TermTyConv ; [ ceapply TermAbs | .. ].
-      * magic.
-      *
-Abort.
+(* We define transport as an extra symbol *)
+Context {transport : nat -> term -> term -> term -> term -> term}.
+Context {
+  TermTransport :
+    forall {Γ n T1 T2 p t},
+      Ttt.isctx Γ ->
+      Ttt.isterm Γ T1 (Uni (uni n)) ->
+      Ttt.isterm Γ T2 (Uni (uni n)) ->
+      Ttt.isterm Γ p (Id (Uni (uni n)) T1 T2) ->
+      Ttt.isterm Γ t T1 ->
+      Ttt.isterm Γ (transport n T1 T2 p t) T2
+}.
 
 End Translation.
